vale/code/lib/transformers/Vale.Transformers.MovbeElim.fst
@@ -1,0 +1,22 @@
+module Vale.Transformers.MovbeElim
+
+open Vale.X64.Bytes_Code_s
+open Vale.X64.Instruction_s
+open Vale.X64.Instructions_s
+open Vale.X64.Machine_Semantics_s
+open Vale.X64.Machine_s
+open Vale.X64.Print_s
+open Vale.Transformers.InstructionReorder
+open Vale.X64.InsLemmas
+
+open Vale.Transformers.PeepHole
+
+let movbe_elim_ph (is:list ins) : Tot (option (list ins)) =
+  None (* Safe, but currently behaves as a no-op due to this *)
+
+let movbe_elim_correct (is:list ins) (s:machine_state) :
+  Lemma (peephole_correct movbe_elim_ph is s)
+    [SMTPat (peephole_correct movbe_elim_ph is s)] =
+  ()
+
+let movbe_elim_input_hint : pos = 1
